Semantic/Consume/TypeSystem/Core.lean
@@ -117,6 +117,7 @@ inductive HasType : CaptureSet s -> Ctx s -> Exp s -> Ty .exi s -> Prop where
 | var :
   Γ.IsClosed ->
   Γ.LookupVar x T ->
+  T.captureSet.accessible Γ ->
   ----------------------------
   HasType
     {}
@@ -176,7 +177,7 @@ inductive HasType : CaptureSet s -> Ctx s -> Exp s -> Ty .exi s -> Prop where
   HasType C Γ t (.exi T) ->
   HasType
     ((C.rename Rename.succ).rename Rename.succ)
-    (Γ,C<:.unbound,x:T)
+    (Γ.push_cvar_consume .unbound,x:T)
     u
     ((U.rename Rename.succ).rename Rename.succ) ->
   --------------------------------------------
